KeyEquivalence.fst
@@ -1,52 +1,6 @@
 module KeyEquivalence
 
-(** Define split and merge primitives. This will let us combine
-    arbitrary [nat]s losslessly. [merge_nat a b] merges [a] and [b]
-    into a single [nat] which has [a] in the higher order digits, and
-    [b] in the lower order digits. [split_nat_a] and [split_nat_b] are
-    used to retrieve [a] and [b] from the merged [nat].
-
-    [merge_split_inverses] tells us that the merge and split functions
-    are inverses of each other. *)
-
-type natlim (lim:pos) = x:nat{x<lim}
-
-val split_nat : #lim:pos -> c:natlim (lim `op_Multiply` lim) ->
-  a:natlim lim * b:natlim lim
-let split_nat #lim c = c / lim, c % lim
-
-val merge_nat : #lim:pos -> a:natlim lim -> b:natlim lim ->
-  c:natlim (lim `op_Multiply` lim)
-let merge_nat #lim a b =
-  let k = (a `op_Multiply` lim) in
-  assert (k <= lim `op_Multiply` (lim - 1));
-  (* This assertion lets it prove that the output limit is correct *)
-  let l = k + b in
-  l
-
-  (* Need to increase limits to prove divmod lemma below *)
-  #set-options "--z3rlimit 20"
-
-
-val divmod_lemma : #lim:pos -> a:natlim lim -> b:natlim lim ->
-  Lemma ((((a `op_Multiply` lim) + b) / lim = a) /\
-         (((a `op_Multiply` lim) + b) % lim = b))
-let divmod_lemma #lim a b =
-  Math.Lemmas.modulo_addition_lemma b lim a
-
-val merge_split_inverses :
-  #lim:pos -> a:natlim lim -> b:natlim lim ->
-  c:natlim (lim `op_Multiply` lim) ->
-  Lemma (
-    (merge_nat a b = c) <==>
-    (split_nat c = (a, b)))
-let merge_split_inverses #lim a b c = divmod_lemma #lim a b
-
-(** Prove equivalence b/w the key types used by the Vale and the HACL*
-    specs. We do this by using the merging and splitting primitives
-    defined above.
-
-    Defines [key_vale_to_hacl] and [key_hacl_to_vale] to convert
+(** Defines [key_vale_to_hacl] and [key_hacl_to_vale] to convert
     between the two keys, and [key_equivalence] lemma proves that they
     are equivalent. *)
 
@@ -56,39 +10,58 @@ module HaclSpec = Spec.Poly1305
 type nat128 = ValeSpec.nat128
 type key = HaclSpec.key
 
-open Spec.Lib.IntSeq
 open Spec.Lib.IntTypes
+open Spec.Lib.IntSeq
+open Axioms
 
 val key_hacl_to_vale : k:key -> r:nat128 * s:nat128
 let key_hacl_to_vale k =
-  let c = nat_from_intseq_le k in
-  Math.Lemmas.pow2_plus 128 128;
-  let a, b = split_nat #(pow2 128) c in
-  b, a
+  let r = slice_semantics k 0 16; slice k 0 16 in
+  let s = slice_semantics k 16 32; slice k 16 32 in
+  nat_from_intseq_le r, nat_from_intseq_le s
 
 val key_vale_to_hacl :
   r:nat128 -> s:nat128 ->
   k:key
 let key_vale_to_hacl r s =
-  let c = merge_nat #(pow2 128) s r in
-  Math.Lemmas.pow2_plus 128 128;
-  nat_to_bytes_le 32 c
+  append
+    (nat_to_bytes_le 16 r)
+    (nat_to_bytes_le 16 s)
 
-let equal_intseqs a b =
-  nat_from_intseq_le a = nat_from_intseq_le b
+val part_inv_hacl :
+  k:key ->
+  Lemma (k ==
+         key_vale_to_hacl
+           (fst (key_hacl_to_vale k))
+           (snd (key_hacl_to_vale k)))
+
+let part_inv_hacl k =
+  let r = slice_semantics k 0 16; slice k 0 16 in
+  let s = slice_semantics k 16 32; slice k 16 32 in
+  let r', s' = nat_from_intseq_le r, nat_from_intseq_le s in
+  assert ((r', s') = key_hacl_to_vale k);
+  let k' = key_vale_to_hacl r' s' in
+  let r0, s0 = sub k' 0 16, sub k' 16 16 in
+  eq_nat_from_intseq r r0;
+  eq_nat_from_intseq s s0;
+  assert (r == r0);
+  assert (s == s0);
+  MsgEquivalence.lemma_subseq #32 #16 #16 k k' // TODO: Move this property into a separate file and then use it here
+
+val part_inv_vale :
+  r:nat128 ->
+  s:nat128 ->
+  Lemma ((r,s) = key_hacl_to_vale (key_vale_to_hacl r s))
+
+let part_inv_vale r s = admit () // TODO: Prove
 
 val key_equivalence :
   r:nat128 ->
   s:nat128 ->
   k:key ->
-  Lemma (
-    (equal_intseqs (key_vale_to_hacl r s) k)
-    <==>
-    (key_hacl_to_vale k == (r, s))
-  )
+  Lemma ((key_vale_to_hacl r s == k) <==>
+         (key_hacl_to_vale k == (r, s)))
 
 let key_equivalence r s k =
-  Math.Lemmas.pow2_plus 128 128;
-  let c = (merge_nat #(pow2 128) r s) in
-  merge_split_inverses r s c
-
+  part_inv_hacl k;
+  part_inv_vale r s
